saw-core-coq: Explicitly define atWithProof, genWithProof, and friends
This provides explicit Coq definitions for SAWCore's `atWithProof` and
`genWithProof` functions, which allow them to compute. It also proves the
auxiliary `at_gen_BVVec` and `gen_at_BVVec` lemmas, a feat which is now possible
thanks to the aforementioned computability.

To make this work with the current module ordering, I needed to wire in the
definition of `IsLtNat` into `SAWCoreScaffolding`, which proves
straightforward.

Fixes #1784.

saw-core-coq/src/Verifier/SAW/Translation/Coq/SpecialTreatment.hs
@@ -337,12 +337,13 @@ sawCorePreludeSpecialTreatmentMap configuration =
   , ("Refl",    mapsToExpl logicModule "eq_refl")
   ]
 
-  -- Nat le
+  -- Nat le/lt
   ++
   [ ("IsLeNat"     , mapsTo sawDefinitionsModule "IsLeNat")
   , ("IsLeNat__rec", mapsTo sawDefinitionsModule "IsLeNat__rec")
   , ("IsLeNat_base", mapsTo sawDefinitionsModule "IsLeNat_base")
   , ("IsLeNat_succ", mapsTo sawDefinitionsModule "IsLeNat_succ")
+  , ("IsLtNat"     , mapsTo sawDefinitionsModule "IsLtNat")
   ]
 
   -- Strings
@@ -370,7 +371,9 @@ sawCorePreludeSpecialTreatmentMap configuration =
   ++
   [ ("EmptyVec",      mapsTo vectorsModule "EmptyVec")
   , ("at",            rename "sawAt") -- `at` is a reserved keyword in Coq
+  , ("at_gen_BVVec",  mapsTo preludeExtraModule "at_gen_BVVec")
   , ("atWithDefault", mapsTo vectorsModule "atWithDefault")
+  , ("atWithProof",   mapsTo vectorsModule "atWithProof")
   , ("at_single",     skip) -- is boring, could be proved on the Coq side
   , ("bvAdd",         mapsTo vectorsModule "bvAdd")
   , ("bvLg2",         mapsTo vectorsModule "bvLg2")
@@ -394,6 +397,8 @@ sawCorePreludeSpecialTreatmentMap configuration =
   , ("eq_Vec",        skip)
   , ("foldr",         mapsTo vectorsModule "foldr")
   , ("foldl",         mapsTo vectorsModule "foldl")
+  , ("gen_at_BVVec",  mapsTo preludeExtraModule "gen_at_BVVec")
+  , ("genWithProof",  mapsTo vectorsModule "genWithProof")
   , ("scanl",         mapsTo vectorsModule "scanl")
   , ("gen",           mapsTo vectorsModule "gen")
   , ("rotateL",       mapsTo vectorsModule "rotateL")
