saw-core-coq/coq/handwritten/CryptolToCoq/SAWCorePreludeExtra.v
@@ -1,10 +1,15 @@
+From Coq          Require Import Arith.Peano_dec.
+From Coq          Require Import Arith.PeanoNat.
 From Coq          Require Import Lists.List.
+From Coq          Require Import Logic.Eqdep_dec.
 From Coq          Require Import Logic.FunctionalExtensionality.
 Import ListNotations.
 From Coq          Require Import String.
 From Coq          Require Import Vectors.Vector.
+From CryptolToCoq Require Import SAWCoreBitvectors.
 From CryptolToCoq Require Import SAWCoreScaffolding.
 From CryptolToCoq Require Import SAWCorePrelude.
+From CryptolToCoq Require Import SAWCoreVectorsAsCoqVectors.
 Import SAWCorePrelude.
 
 Fixpoint Nat_cases2_match a f1 f2 f3 (x y : nat) : a :=
@@ -66,6 +71,60 @@ Lemma streamScanl_succ a b f z xs : forall n,
     (streamGet a xs n).
 Proof.
   intro n. reflexivity.
+Qed.
+
+Lemma bvToNat_bvNat (w n : nat) :
+  n < 2^w -> bvToNat w (bvNat w n) = n.
+Admitted.
+
+Lemma bvToNat_bounds (w : nat) (x : bitvector w) :
+  bvToNat w x < 2^w.
+Proof.
+  holds_for_bits_up_to_3; try repeat constructor.
+Qed.
+
+Theorem at_gen_BVVec :
+  forall (n : nat) (len : bitvector n) (a : Type)
+         (f : forall i : bitvector n, is_bvult n i len -> a)
+         (ix : bitvector n) (pf : is_bvult n ix len),
+  atBVVec n len a (genBVVec n len a f) ix pf = f ix pf.
+Proof.
+  intros n len a f ix pf.
+  unfold atBVVec, genBVVec.
+  rewrite at_gen_Vec.
+  generalize (IsLtNat_to_bvult n len (bvToNat n ix)
+               (bvult_to_IsLtNat n len (bvToNat n ix)
+                 (trans bool (bvult n (bvNat n (bvToNat n ix)) len) (bvult n ix len) 1%bool
+                   (eq_cong (bitvector n) (bvNat n (bvToNat n ix)) ix (bvNat_bvToNat n ix) bool
+                     (fun y : bitvector n => bvult n y len)) pf))) as pf2.
+  rewrite (bvNat_bvToNat n ix).
+  intros pf2.
+  rewrite (UIP_dec Bool.bool_dec pf2 pf).
+  reflexivity.
+Qed.
+
+Lemma gen_at_BVVec :
+  forall (n : nat) (len : bitvector n) (a : Type) (x : BVVec n len a),
+  genBVVec n len a (atBVVec n len a x) = x.
+Proof.
+  intros n len a x.
+  unfold genBVVec, atBVVec.
+  rewrite <- (gen_at_Vec _ _ x) at 1.
+  f_equal. extensionality i. extensionality pf.
+  generalize (bvult_to_IsLtNat n len (bvToNat n (bvNat n i))
+               (trans bool (bvult n (bvNat n (bvToNat n (bvNat n i))) len) (bvult n (bvNat n i) len) 1%bool
+                 (eq_cong (bitvector n) (bvNat n (bvToNat n (bvNat n i))) (bvNat n i)
+                    (bvNat_bvToNat n (bvNat n i)) bool (fun y : bitvector n => bvult n y len))
+                 (IsLtNat_to_bvult n len i pf))) as pf2.
+  assert (X : bvToNat n (bvNat n i) = i).
+  { apply bvToNat_bvNat.
+    transitivity (bvToNat n len).
+    - exact pf.
+    - apply bvToNat_bounds.
+  }
+  rewrite X. intros pf2.
+  rewrite (le_unique _ _ pf2 pf).
+  reflexivity.
 Qed.
 
 
